# Why the differences from the mean must add to zero.

Have a look at this little bit of algebra to see why.

Imagine I have four values $a, b, c, d$.

Call the mean $\mu$. As we know:

$$
\mu = (a + b + c + d) / 4
$$

Now subtract $\mu$ from every one of $a, b, c, d$, and add up the result. We
get;

$$
a - \mu + \\
b - \mu + \\
c - \mu + \\
d - \mu = \\
(a + b + c + d) - 4 \mu
$$

But:

$$
4 \mu = \\
4 (a + b + c + d) / 4 \\
= a + b + c + d
$$

So:

$$
a - \mu + \\
b - \mu + \\
c - \mu + \\
d - \mu = \\
(a + b + c + d) - 4 \mu = \\
(a + b + c + d) - (a + b + c + d) = \\
0
$$
